tactic now solves the goals in BabySep.

src/SepIL.v
@@ -143,6 +143,15 @@ Export ST.HT.
 Require SepExpr.
 Module SEP := SepExpr.SepExpr BedrockHeap ST.
 
+Definition bedrock_types : list Expr.type :=
+  (** TODO: I think that we want a comparable W **)
+  {| Expr.Impl := W 
+   ; Expr.Eq := fun x y => 
+     match weq x y with
+       | left pf => Some pf 
+       | _ => None 
+     end |} :: Expr.defaultType (settings * state)%type :: nil.
+
 (** * Define some convenient connectives, etc. for specs *)
 
 Definition memoryIn : W -> mem -> smem := memoryIn (width := 32).
@@ -207,6 +216,50 @@ Definition Himp (p1 p2 : HProp) : Prop :=
   forall specs, ST.himp specs p1 p2.
 
 Notation "p1 ===> p2" := (Himp p1%Sep p2%Sep) (no associativity, at level 90).
+
+(*
+Lemma ApplyCancelSep : forall types funcs sfuncs l r,
+  (forall cs,
+    match SEP.CancelSep (funcs := funcs) (sfuncs := sfuncs) cs nil l r with
+      | SEP.Prove vars u2 l' r' SUBST _ =>
+        SEP.forallEach
+        (fun VS : hlist (@Expr.tvarD (bedrock_types ++ types)) vars =>
+          SEP.exists_subst VS SUBST
+          (fun k : hlist (@Expr.tvarD (bedrock_types ++ types)) u2 => SEP.himp HNil k VS cs l' r'))
+    end) ->
+  (SEP.sexprD (pcType := Expr.tvTrans FO) (stateType := Expr.tvTrans (FS FO)) l HNil HNil)
+  ===>
+  (SEP.sexprD (pcType := Expr.tvTrans FO) (stateType := Expr.tvTrans (FS FO)) r HNil HNil).
+Proof.
+  unfold Himp. intros. specialize (H specs). 
+  apply SEP.ApplyCancelSep in H. unfold SEP.himp in *. assumption.
+Qed.
+*)
+
+Lemma Himp_to_SEP_himp : forall types funcs sfuncs 
+  (l r : @SEP.sexpr (bedrock_types ++ types) funcs (Expr.tvTrans FO) (Expr.tvTrans (FS FO)) sfuncs nil nil),
+  (forall cs, 
+    SEP.himp HNil HNil HNil cs l r) ->
+  SEP.sexprD l HNil HNil ===> SEP.sexprD r HNil HNil.
+Proof.
+  unfold Himp, SEP.himp. intuition.
+Qed.
+
+Ltac reflect_goal isConst Ts :=
+  match goal with 
+    | [ |- Himp ?L ?R ] =>
+      let pcT := constr:(W) in
+      let stateT := constr:(prod settings state) in
+      let Ts := eval unfold bedrock_types in bedrock_types in
+      let goals := constr:(L :: R :: nil) in
+      let goals := eval unfold starB exB hvarB in goals in
+      let v := SEP.reflect_all pcT stateT ltac:(isConst) Ts goals in
+      match v with
+        | (?L, (?R, _)) => 
+          idtac L ; idtac R ; 
+          eapply (@Himp_to_SEP_himp _ _ _ L R)
+      end
+  end.
 
 (** * The main injector of separation formulas into PropX *)
 
